allocator/slabs bottom-up 7/n
some cleaning
before wiring up allocate_small
and C bindings

alloc/Slabs.fst
@@ -1,6 +1,5 @@
 module Slabs
 
-module L = FStar.List.Tot
 open Steel.Effect.Atomic
 open Steel.Effect
 module A = Steel.Array
@@ -11,10 +10,9 @@ module I64 = FStar.Int64
 module I32 = FStar.Int32
 module U8 = FStar.UInt8
 
-module M = FStar.Math.Lib
 module G = FStar.Ghost
 module FU = FStar.UInt
-open Seq2
+module L = FStar.List.Tot
 
 let array = Steel.ST.Array.array
 let ptr = Steel.ST.Array.ptr
@@ -22,31 +20,36 @@ let ptr = Steel.ST.Array.ptr
 open FStar.Mul
 open Utils
 
-let array_to_bv_slice
-  (#n: nat)
-  (s0: Seq.lseq U64.t n)
-  (i: nat)
-  : Lemma
-  (requires
-    i < n
-  )
-  (ensures (
-    let bm0 = Bitmap4.array_to_bv2 s0 in
-    let x = Seq.index s0 i in
-    Seq.slice bm0 (i*64) ((i+1)*64)
-    =
-    FU.to_vec #64 (U64.v x)))
-  =
-  Bitmap4.array_to_bv_lemma_upd_set_aux4 s0 (i*64)
-
 //TODO: should not be hardcoded
 let page_size = 4096ul
+let slab_max_number = 4096ul
+
+noextract
+let min_sc = 16
+noextract
+let max_sc = 64
 
 //TODO: second constraint should be relaxed
 //currently does not support size classes with <64 slots
 //that require a subtle loop to read only possible
 //corresponding slots in the bitmap
-let sc = x:U32.t{16 <= U32.v x /\ U32.v x <= 64}
+let sc = x:U32.t{min_sc <= U32.v x /\ U32.v x <= max_sc}
+
+let slab_region_len : U32.t = normalize_term (U32.mul page_size slab_max_number)
+unfold let slab_region
+  = r:array U8.t{A.length r = U32.v slab_region_len}
+
+let slab_md_region_len : U32.t = normalize_term (U32.mul 40ul slab_max_number)
+unfold let slab_md_region
+  = r:array U8.t{A.length r = U32.v slab_md_region_len}
+
+// C binding, no top-level Steel initialization
+assume val get_slab_region (_:unit)
+  : slab_region
+
+// C binding, no top-level Steel initialization
+assume val get_slab_md_region (_:unit)
+  : slab_md_region
 
 let nb_slots (size_class: sc)
   : Pure U32.t
@@ -57,6 +60,12 @@ let nb_slots (size_class: sc)
   )
   =
   U32.div page_size size_class
+
+//TODO
+noextract
+let slab_md_bitmap_length = nb_slots (U32.uint_to_t min_sc)
+
+unfold let slab_metadata = r:array U64.t{A.length r = 4}
 
 #push-options "--z3rlimit 30"
 inline_for_extraction noextract
@@ -92,7 +101,6 @@ let get_free_slot_aux
   let r' = U32.mul 64ul i in
   U32.add r r'
 #pop-options
-
 
 noextract
 let has_free_slot
@@ -141,12 +149,6 @@ let get_free_slot (size_class: sc) (bitmap: slab_metadata)
     get_free_slot_aux size_class bitmap 0ul
   )
 
-
-let starl (l: list vprop)
-  : vprop
-  =
-  L.fold_left star emp l
-
 #push-options "--z3rlimit 20"
 let slot_array (size_class: sc) (arr: array U8.t) (pos: U32.t)
   : Pure (array U8.t)
@@ -177,19 +179,6 @@ let array_slot (size_class: sc) (arr: array U8.t) (slot: array U8.t)
   let offset_bytes = A.offset ptr2 - A.offset ptr1 in
   let offset_slot = offset_bytes / (U32.v size_class) in
   offset_slot
-
-let lemma_div (x y z: nat)
-  : Lemma
-  (requires
-    x = y * z /\
-    z > 0
-  )
-  (ensures
-    x / z = y
-  )
-  =
-  FStar.Math.Lemmas.lemma_mod_plus 0 y z;
-  assert ((y * z) % z = 0)
 
 let array_slot_slot_array_bij (size_class: sc) (arr: array U8.t) (pos: U32.t)
   : Lemma
@@ -241,12 +230,6 @@ let slab_vprop3 (size_class: sc) (arr: array U8.t{A.length arr = U32.v page_size
   let r = slab_vprop2 size_class arr s in
   starl r
 
-let lemma_seq_to_list_append (#a:Type) (s1 s2: Seq.seq a)
-  : Lemma
-  (Seq.seq_to_list (Seq.append s1 s2) == L.append (Seq.seq_to_list s1) (Seq.seq_to_list s2))
-  =
-  admit ()
-
 let slab_vprop2_lemma
   (size_class: sc) (arr: array U8.t{A.length arr = U32.v page_size})
   (s1 s2: Seq.seq (r:nat{r < U32.v (nb_slots size_class)}))
@@ -263,12 +246,6 @@ let slab_vprop2_lemma
   lemma_seq_to_list_append
     (slab_vprop1 size_class arr s1)
     (slab_vprop1 size_class arr s2)
-
-// TODO @AF
-let starl_append (l1 l2: list vprop)
-  : Lemma
-  (starl (L.append l1 l2) `equiv` (starl l1 `star` starl l2))
-  = admit ()
 
 let slab_vprop3_lemma
   (size_class: sc) (arr: array U8.t{A.length arr = U32.v page_size})
@@ -293,16 +270,6 @@ let slab_vprop
   =
   let s = Seq.slice (Seq.init (U32.v (nb_slots size_class)) (fun k -> k)) i j in
   slab_vprop3 size_class arr s
-
-let lemma_index_slice (#a:Type) (s:Seq.seq a)
-  (i:nat)
-  (j:nat{i <= j /\ j <= Seq.length s})
-  (k:nat{k < j - i})
-  : Lemma
-  (requires True)
-  (ensures (Seq.index (Seq.slice s i j) k == Seq.index s (k + i)))
-  =
-  Seq.lemma_index_slice s i j k
 
 let slab_vprop_lemma
   (size_class: sc)
@@ -446,81 +413,6 @@ let allocate_slot (size_class: sc)
   return (G.hide (U32.v slot_pos), slot)
 
 (*)
-  let slab_vprop_sl_lemma (m: SM.mem)
-    : Lemma
-    (requires SM.interp (hp_of (
-      (slab_vprop size_class arr 0 (nb_slots size_class) `star` A.varray md)
-    )) m)
-    (ensures SM.interp (hp_of (
-      (slab_vprop size_class arr 0 i `star`
-      slab_vprop size_class arr i (nb_slots size_class) `star`
-      A.varray md)
-    )) m)
-    =
-    slab_vprop_lemma size_class arr 0 i (nb_slots size_class)
-  in
-  rewrite_slprop
-    (slab_vprop size_class arr 0 (nb_slots size_class) `star`
-    A.varray md)
-    (slab_vprop size_class arr 0 i `star`
-    slab_vprop size_class arr i (nb_slots size_class) `star`
-    A.varray md)
-    (fun m -> slab_vprop_sl_lemma m);
-  //slab_vprop_lemma size_class arr 0 (U32.v slot_pos) (nb_slots size_class);
-  sladmit ();
-  return slot
-
-(*)
-
-
-    (bm_to_vprop #128 32 md)
-    (A.varray (get_slab_region ()) `star`
-    A.varray md)
-    (fun a -> A.varray (get_slab_region ()) `star`
-    A.varray md)
-    (fun _ -> U32.v len = 32)
-    (fun _ r h1 ->
-      True
-    )
-  =
-  let a = get_slab_region () in
-  let slot = get_free_slot md in
-  Bitmap5.bm_set #4 md slot;
-  let offset = U32.mul 32ul slot in
-  let ptr_slab_region = A.ptr_of a in
-      )
-    ) else (
-      let idx =
-    )
-  ) else (
-
-  )
-  admit ();
-  0ul
-
-
-
-
-let allocate_small (len: U32.t) (md: slab_metadata)
-  : Steel (ptr U8.t)
-    (A.varray (get_slab_region ()) `star`
-    A.varray md)
-    (fun a -> A.varray (get_slab_region ()) `star`
-    A.varray md)
-    (fun _ -> U32.v len = 32)
-    (fun _ r h1 ->
-      True
-    )
-  =
-  let a = get_slab_region () in
-  let slot = get_free_slot md in
-  Bitmap5.bm_set #4 md slot;
-  let offset = U32.mul 32ul slot in
-  let ptr_slab_region = A.ptr_of a in
-  let ptr = A.ptr_shift ptr_slab_region offset in
-  return ptr
-
-(*)
 //noextract
 //let size_classes : list nzn = [
 //  //(* 0 *) 0;
@@ -548,356 +440,3 @@ let nb_slots (x: nzn) : nzn = U32.div page_size x
 
 let slab_metadata (size_class: nzn)
   = Seq.lseq bool (U32.v (nb_slots size_class))
-
-// used outside of spec, hence the u32
-let ptr_slot
-  (size_class: nzn)
-  (slab: slab{A.is_full_array slab})
-  (n: U32.t{U32.lt n (nb_slots size_class)})
-  : A.ptr U8.t
-  =
-  let ptr_slab = dfst slab in
-  let shift = U32.mul n size_class in
-  let ptr_slot = A.ptr_shift ptr_slab shift in
-  ptr_slot
-
-let arr_slot
-  (size_class: nzn)
-  (slab: slab{A.is_full_array slab})
-  (n: U32.t{U32.lt n (nb_slots size_class)})
-  : arr:array U8.t{A.length arr = U32.v size_class}
-  =
-  let ptr = ptr_slot size_class slab n in
-  let length = G.hide (U32.v size_class) in
-  (| ptr, length |)
-
-//@Spec
-noextract
-let init_nat (len: nat)
-  : Seq.lseq (k:nat{k < len}) len
-  = Seq.init len (fun k -> k)
-//@Spec
-noextract
-let init_u32 (len: U32.t)
-  : Seq.lseq (k:U32.t{U32.v k < U32.v len}) (U32.v len)
-  =
-  let s : Seq.lseq (k:nat{k < U32.v len}) (U32.v len)
-    = init_nat (U32.v len) in
-  let f : k:nat{k < U32.v len} -> k':U32.t{U32.v k' < U32.v len}
-    = fun k -> U32.uint_to_t k in
-  Seq.map_seq_len f s;
-  Seq.map_seq f s
-//@Spec
-noextract
-let slab_to_slots
-  (size_class: nzn)
-  (slab: slab{A.is_full_array slab})
-  : Seq.lseq
-    (arr:array U8.t{A.length arr = U32.v size_class})
-    (U32.v (nb_slots size_class))
-  =
-  let n = nb_slots size_class in
-  let s = init_u32 n in
-  let f = fun (k:U32.t{U32.v k < U32.v n})
-          -> arr_slot size_class slab k in
-  Seq.map_seq_len f s;
-  Seq.map_seq f s
-//@Spec
-noextract
-let sl_state
-  (size_class: nzn)
-  (slab: slab{A.is_full_array slab})
-  (slab_md: slab_metadata size_class)
-  : Seq.lseq vprop (U32.v (nb_slots size_class))
-  =
-  let f : bool -> array U8.t -> vprop
-    = fun b arr -> if b then A.varray arr else emp in
-  let s1 = slab_md in
-  let s2 = slab_to_slots size_class slab
-  in
-  map_seq2_len f s1 s2;
-  map_seq2 f s1 s2
-//@Spec
-let set_alloc
-  (size_class: nzn)
-  (slab_md: slab_metadata size_class)
-  (i:nat{i < Seq.length slab_md})
-  : Pure (slab_metadata size_class)
-  (requires Seq.index slab_md i = false)
-  (ensures fun slab_md' ->
-    Seq.index slab_md' i = true /\
-    (forall j. j <> i ==> Seq.index slab_md' j == Seq.index slab_md j)
-  )
-  = Seq.upd slab_md i true
-//@Spec
-let set_free
-  (size_class: nzn)
-  (slab_md: slab_metadata size_class)
-  (i:nat{i < Seq.length slab_md})
-  : Pure (slab_metadata size_class)
-  (requires Seq.index slab_md i = true)
-  (ensures fun slab_md' ->
-    Seq.index slab_md' i = false /\
-    (forall j. j <> i ==> Seq.index slab_md' j == Seq.index slab_md j)
-  )
-  = Seq.upd slab_md i false
-
-let div_nbn_is_n (x y: int)
-  : Lemma
-  (requires x >= 0 /\ y > 0)
-  (ensures x / y >= 0)
-  = ()
-
-noextract
-let spec_smd_index_op0
-  (size_class: nzn{U32.v size_class >= 16})
-  (slab_md: Seq.lseq U64.t 4)
-  (i: U32.t{U32.lt i (nb_slots size_class)})
-  : U64.t
-  =
-  assert (U32.lte (nb_slots size_class) 256ul);
-  let bucket_pos = U32.v i / 64 in
-  assert (bucket_pos < 4);
-  let bucket = Seq.index slab_md bucket_pos in
-  bucket
-
-//@Spec
-//open FStar.UInt
-let uint64_to_uint32 (x: U64.t) (bound: nat)
-  : Pure U32.t
-  (requires U64.v x < bound /\ bound < FStar.UInt.max_int 32)
-  (ensures fun r -> U32.v r == U64.v x /\ U32.v r < bound)
-  = FStar.Int.Cast.uint64_to_uint32 x
-open BVL
-
-let smd_index_op0
-  (size_class: nzn{U32.v size_class >= 16})
-  (slab_md: array U64.t{A.length slab_md == 4})
-  (i: U32.t{U32.lt i (nb_slots size_class)})
-  : Steel U64.t
-  (A.varray slab_md)
-  (fun _ -> A.varray slab_md)
-  (requires fun h0 -> True)
-  (ensures fun h0 x h1 ->
-    A.asel slab_md h1 == A.asel slab_md h0 /\
-    x == spec_smd_index_op0 size_class (A.asel slab_md h1) i
-  )
-  =
-  assert (U32.lte (nb_slots size_class) 256ul);
-  assert (U32.v i < 256);
-  let i64 = uint32_to_uint64 i in
-  let bucket_pos = div64_shift i64 in
-  assert (U64.v bucket_pos < 4);
-  let bucket_pos = uint64_to_uint32 bucket_pos 4 in
-  let bucket = A.index slab_md bucket_pos in
-  bucket
-
-//@Spec
-open FStar.Mul
-noextract
-let spec_smd_index_op1
-  (size_class: nzn{U32.v size_class >= 16})
-  (bucket: U64.t)
-  (i: U32.t{U32.lt i (nb_slots size_class)})
-  : nat
-  =
-  assert (U32.lte (nb_slots size_class) 256ul);
-  assert (U32.v i < 256);
-  let bucket_pos = U32.v i / 64 in
-  assert (bucket_pos < 4);
-  let mask_shift : nat = U32.v i - (bucket_pos * 64) in
-  assert (mask_shift = U32.v i % 64);
-  mask_shift
-
-let smd_index_op1
-  (size_class: nzn{U32.v size_class >= 16})
-  (bucket: U64.t)
-  (i: U32.t{U32.lt i (nb_slots size_class)})
-  : r:U32.t{U32.v r < 64}
-  =
-  assert (U32.lte (nb_slots size_class) 256ul);
-  assert (U32.v i < 256);
-  let i64 = uint32_to_uint64 i in
-  assert (U64.v i64 == U32.v i);
-  let bucket_pos = div64_shift i64 in
-  assert (U64.v bucket_pos = U32.v i / 64);
-  assert (U64.v bucket_pos < 4);
-  let mask_shift_aux = mul64_shift bucket_pos in
-  assert (U64.v mask_shift_aux = 64 * U64.v bucket_pos);
-  let mask_shift = U64.sub i64 mask_shift_aux in
-  assert (U64.v mask_shift = (U32.v i) % 64);
-  assert (U64.v mask_shift < 64);
-  let mask_shift32 : k:U32.t{U32.v k < 64}
-    = uint64_to_uint32 mask_shift 64 in
-  mask_shift32
-
-let equiv_smd_index_op1
-  (size_class: nzn{U32.v size_class >= 16})
-  (bucket: U64.t)
-  (i: U32.t{U32.lt i (nb_slots size_class)})
-  : Lemma
-  (
-  let r11 = spec_smd_index_op1 size_class bucket i in
-  let r21 = smd_index_op1 size_class bucket i in
-  r11 = U32.v r21)
-  = ()
-
-noextract
-let spec_smd_index_op2
-  (size_class: nzn{U32.v size_class >= 16})
-  (bucket: U64.t)
-  (mask_shift: nat)
-  : bool
-  =
-  div_nbn_is_n (U64.v bucket) (pow2  mask_shift);
-  let r : nat = (U64.v bucket) / (pow2 mask_shift) in
-  if r % 2 = 1
-  then true
-  else false
-
-let smd_index_op2
-  (size_class: nzn{U32.v size_class >= 16})
-  (bucket: U64.t)
-  (mask_shift: U32.t{U32.v mask_shift < 64})
-  : bool
-  =
-  let r = div64_shift2 bucket mask_shift in
-  assert (U64.v r == (U64.v bucket) / (pow2 (U32.v mask_shift)));
-  let r = U64.logand r 1UL in
-  if U64.eq r 1UL
-  then true
-  else false
-
-let equiv_smd_index_op2
-  (size_class: nzn{U32.v size_class >= 16})
-  (bucket: U64.t)
-  (mask_shift: U32.t{U32.v mask_shift < 64})
-  : Lemma
-  (
-  let r11 = spec_smd_index_op2 size_class bucket (U32.v mask_shift) in
-  let r21 = smd_index_op2 size_class bucket mask_shift in
-  r11 = r21)
-  =
-  Classical.forall_intro logand1
-
-noextract
-let spec_smd_index_op3
-  (size_class: nzn{U32.v size_class >= 16})
-  (bucket: U64.t)
-  (mask_shift: nat)
-  : nat
-  =
-  let r = (U64.v bucket) + (pow2 mask_shift) in
-  r
-
-let smd_index_op3
-  (size_class: nzn{U32.v size_class >= 16})
-  (bucket: U64.t)
-  (mask_shift: U32.t{U32.v mask_shift < 64})
-  : U64.t
-  =
-  let shifted_one = mul64_shift2 mask_shift in
-  assert (U64.v shifted_one ==  pow2 (U32.v mask_shift));
-  let r = U64.logor bucket shifted_one in
-  r
-
-
-
-//@Spec
-noextract
-let spec_smd_index
-  (size_class: nzn{U32.v size_class >= 16})
-  (slab_md: Seq.lseq U64.t 4)
-  (i: U32.t{U32.lt i (nb_slots size_class)})
-  : bool
-  =
-  let bucket = spec_smd_index_op0 size_class slab_md i in
-  let mask_shift = spec_smd_index_op1 size_class bucket i in
-  let r = spec_smd_index_op2 size_class bucket mask_shift in
-  r
-
-let smd_index
-  (size_class: nzn{U32.v size_class >= 16})
-  (slab_md: array U64.t{A.length slab_md == 4})
-  (i: U32.t{U32.lt i (nb_slots size_class)})
-  : Steel bool
-  (A.varray slab_md)
-  (fun _ -> A.varray slab_md)
-  (requires fun h0 -> True)
-  (ensures fun h0 b h1 ->
-      b == spec_smd_index size_class (A.asel slab_md h1) i /\
-      A.asel slab_md h1 == A.asel slab_md h0
-  )
-  =
-  let bucket = smd_index_op0 size_class slab_md i in
-  let mask_shift = smd_index_op1 size_class bucket i in
-  equiv_smd_index_op1 size_class bucket i;
-  let r = smd_index_op2 size_class bucket mask_shift in
-  equiv_smd_index_op2 size_class bucket mask_shift;
-  return r
-
-//@Spec
-noextract
-let smd2b
-  (size_class: nzn{U32.v size_class >= 16})
-  (slab_md: Seq.lseq U64.t 4)
-  : (Seq.lseq bool (U32.v (nb_slots size_class)))
-  =
-  let f = spec_smd_index size_class slab_md in
-  let s1 = init_u32 (nb_slots size_class) in
-  Seq.map_seq_len f s1;
-  Seq.map_seq f s1
-
-[@@__steel_reduce__]
-noextract
-let v_smd
-  (#vp:vprop)
-  (size_class: nzn{U32.v size_class >= 16})
-  (slab_md: array U64.t{A.length slab_md == 4})
-  (h:rmem vp{
-    FStar.Tactics.with_tactic selector_tactic
-      (can_be_split vp (A.varray slab_md) /\ True)
-  })
-  : GTot (Seq.lseq bool (U32.v (nb_slots size_class)))
-  =
-  let s : G.erased (Seq.lseq U64.t 4) = h (A.varray slab_md) in
-  G.hide (smd2b size_class (G.reveal s))
-
-(*)
-
-
-let slab_md_array_set_alloc
-  (size_class: nzn{U32.v size_class >= 16})
-  (slab_md: array U64.t{A.length slab_md == 4})
-  (i: U32.t{U32.lt i (nb_slots size_class)})
-  : Steel unit
-  (A.varray slab_md)
-  (fun _ -> A.varray slab_md)
-  (requires fun h0 -> True)
-  (ensures fun h0 _ h1 ->
-
-  )
-
-
-
-(*)
-
-let slab_md_array_to_seq
-  (size_class: nzn{U32.v size_class >= 16})
-  (slab_md: array U64.t{A.length slab_md == 4})
-  //: slab_metadata size_class
-  : unit
-  = ()
-
-
-(*)
-let get_slot (page: array U8.t) (size_class: nat) (pos: nat)
-  : Steel (array U8.t)
-    (A.varray page)
-    (fun r -> A.varray r)
-    (fun h0 ->
-      A.length page == page_size
-    )
-    (fun h0 r h1 -> A.length r == size_class)
-    =
-    return page
